checkpoint circular_proof
specs seem plausible, proofs seem OK but some annoying parts are
admitted away

src/program_proof/wal/abstraction.v
@@ -52,5 +52,6 @@ Definition is_block (s:Slice.t) (b:Block) :=
 Definition updates_slice (bk_s: Slice.t) (bs: list update.t): iProp Σ :=
   ∃ bks, is_slice_small bk_s (struct.t Update.S) 1 (update_val <$> bks) ∗
    [∗ list] _ ↦ b_upd;upd ∈ bks;bs , let '(update.mk a b) := upd in
-                                     is_block (snd b_upd) b.
+                                     is_block (snd b_upd) b ∗
+                                     ⌜fst b_upd = a⌝.
 End heap.
