src/program_proof/wal/circular_proof.v
@@ -10,6 +10,42 @@ From Perennial.Helpers Require Import GenHeap.
 From Perennial.Helpers Require Import Transitions.
 Existing Instance r_mbind.
 
+
+Section ghost_var_helpers.
+Context {A: ofeT} `{@LeibnizEquiv _ A.(ofe_equiv)} `{OfeDiscrete A}.
+Context {Σ} {Hin: inG Σ (authR (optionUR (exclR A)))}.
+
+Lemma ghost_var_alloc (a: A) :
+  (|==> ∃ γ, own γ (● (Excl' a)) ∗ own γ (◯ (Excl' a)))%I.
+Proof using H0.
+  iMod (own_alloc (● (Excl' a) ⋅ ◯ (Excl' a))) as (γ) "[H1 H2]".
+  { apply auth_both_valid; split; eauto. econstructor. }
+  iModIntro. iExists γ. iFrame.
+Qed.
+
+Lemma ghost_var_agree γ (a1 a2: A) :
+  own γ (● (Excl' a1)) -∗ own γ (◯ (Excl' a2)) -∗ ⌜ a1 = a2 ⌝.
+Proof using H H0.
+  iIntros "Hγ1 Hγ2".
+  iDestruct (own_valid_2 with "Hγ1 Hγ2") as "H".
+  iDestruct "H" as %[<-%Excl_included%leibniz_equiv _]%auth_both_valid.
+  done.
+Qed.
+
+Lemma ghost_var_update γ (a1' a1 a2 : A) :
+  own γ (● (Excl' a1)) -∗ own γ (◯ (Excl' a2)) ==∗
+    own γ (● (Excl' a1')) ∗ own γ (◯ (Excl' a1')).
+Proof.
+  iIntros "Hγ● Hγ◯".
+  iMod (own_update_2 _ _ _ (● Excl' a1' ⋅ ◯ Excl' a1') with "Hγ● Hγ◯") as "[$$]".
+  { by apply auth_update, option_local_update, exclusive_local_update. }
+  done.
+Qed.
+
+End ghost_var_helpers.
+
+
+
 Definition LogSz := 511.
 
 Module circΣ.
@@ -39,16 +75,16 @@ Definition circ_advance (newStart : u64) : transition circΣ.t unit :=
   modify (fun σ => set upds (skipn (Z.to_nat (int.val newStart - int.val σ.(start))%Z)) σ);;
   modify (set start (fun _ => newStart)).
 
-Definition circ_append (l : list update.t) (newend : u64) (lowaddrs : list u64) : transition circΣ.t unit :=
-  assert (fun σ => ∀ (i : nat) u,
-            σ.(upds) !! i = Some u →
-            lowaddrs !! Z.to_nat ((int.val σ.(start) + i) `mod` LogSz)%Z = Some u.(update.addr));;
+Definition circ_append (l : list update.t) (endpos : u64) : transition circΣ.t unit :=
+  assert (fun σ => int.val σ.(start) + length σ.(upds) = int.val endpos);;
   modify (set circΣ.upds (fun u => u ++ l));;
-  assert (fun σ => int.val σ.(start) + length σ.(upds) = int.val newend);;
   assert (fun σ => length σ.(upds) <= LogSz).
+
+Canonical Structure updateC := leibnizO update.t.
 
 Section heap.
 Context `{!heapG Σ}.
+Context `{!inG Σ (authR (optionUR (exclR (listO updateC))))}.
 
 Context (N: namespace).
 Context (P: circΣ.t -> iProp Σ).
@@ -63,25 +99,26 @@ Definition is_low_state (startpos endpos : u64) (updarray : list update.t) : iPr
     ⌜Block_to_vals hdr2 = b2val <$> encode [EncUInt64 startpos] ++ hdr2extra⌝ ∗
     2 d↦∗ (update.b <$> updarray).
 
-Definition is_circular_state (σ : circΣ.t) : iProp Σ :=
-  ∃ updarray,
+Definition is_circular_state γ (σ : circΣ.t) : iProp Σ :=
+  ∃ (updarray : list update.t),
+    own γ (● (Excl' updarray)) ∗
     is_low_state σ.(start) (word.add σ.(start) (length σ.(upds))) updarray ∗
     [∗ list] i ↦ bupd ∈ σ.(upds),
       ⌜updarray !! Z.to_nat ((int.val σ.(start) + i) `mod` LogSz)%Z = Some bupd⌝.
 
-Definition is_circular : iProp Σ :=
-  inv N (∃ σ, is_circular_state σ ∗ P σ).
+Definition is_circular γ : iProp Σ :=
+  inv N (∃ σ, is_circular_state γ σ ∗ P σ).
 
-Definition is_circular_appender (circ: loc) addrList : iProp Σ :=
-  ∃ (diskaddr:loc) s,
-    circ ↦[circularAppender.S :: "diskAddrs"] #diskaddr ∗
-    diskaddr ↦[slice.T uint64T] (slice_val s) ∗
-    is_slice s uint64T 1%Qp ((fun (x : u64) => #x) <$> addrList).
+Definition is_circular_appender γ (circ: loc) : iProp Σ :=
+  ∃ s (updarray : list update.t),
+    own γ (◯ (Excl' updarray)) ∗
+    circ ↦[circularAppender.S :: "diskAddrs"] (slice_val s) ∗
+    is_slice_small s uint64T 1%Qp (u64val <$> (update.addr <$> updarray)).
 
 Opaque encode.
 
-Theorem wp_circular__Advance (Q: iProp Σ) d (newStart : u64) :
-  {{{ is_circular ∗
+Theorem wp_circular__Advance (Q: iProp Σ) γ d (newStart : u64) :
+  {{{ is_circular γ ∗
     (∀ σ, P σ -∗
       ( (∃ σ' b, ⌜relation.denote (circ_advance newStart) σ σ' b⌝) ∧
         (∀ σ' b, ⌜relation.denote (circ_advance newStart) σ σ' b⌝ ={⊤ ∖↑ N}=∗ P σ' ∗ Q)))
@@ -115,7 +152,7 @@ Opaque encode.
 
     iInv N as ">Hcircopen" "Hclose".
     iDestruct "Hcircopen" as (σ) "[Hcs HP]".
-    iDestruct "Hcs" as (updarray) "[Hlow Hupds]".
+    iDestruct "Hcs" as (updarray) "(Hγ & Hlow & Hupds)".
     iDestruct "Hlow" as "[% Hlow]".
     iDestruct "Hlow" as (hdr1 hdr2 hdr2extra) "(Hd0 & Hd1 & % & % & Hd2)".
     iExists _. iFrame.
@@ -137,6 +174,7 @@ Opaque encode.
 
     iNext. iExists _. iFrame.
     iExists _. destruct σ. rewrite /=.
+    iSplitL "Hγ"; first iFrame.
     iSplitL "Hd0 Hd1 Hd2".
     { rewrite /is_low_state. iSplitR "Hd0 Hd1 Hd2".
       2: {
@@ -165,20 +203,187 @@ Opaque encode.
   iFrame.
 Admitted.
 
-Theorem wp_circular__Append (Q: iProp Σ) d (newEnd : u64) (bufs : Slice.t) (upds : list update.t) c (circAppenderList : list u64) :
-  {{{ is_circular ∗
+Fixpoint apply_updates (updarray : list update.t) (endpos : Z) (newupds : list update.t) : list update.t :=
+  match newupds with
+  | u :: newupds' =>
+    <[ Z.to_nat (endpos `mod` LogSz)%Z := u ]> (apply_updates updarray (endpos+1) newupds')
+  | nil => updarray
+  end.
+
+Theorem wp_circularAppender__logBlocks γ c d (endpos : u64) (bufs : Slice.t) (updarray : list update.t) diskaddrslice (upds : list update.t) :
+  {{{ is_circular γ ∗
+      own γ (◯ (Excl' updarray)) ∗
+      c ↦[circularAppender.S :: "diskAddrs"] (slice_val diskaddrslice) ∗
+      is_slice_small diskaddrslice uint64T 1%Qp (u64val <$> (update.addr <$> updarray)) ∗
+      updates_slice bufs upds }}}
+    circularAppender__logBlocks #c #d #endpos (slice_val bufs)
+  {{{ updarray', RET #();
+      own γ (◯ (Excl' updarray')) ∗
+      c ↦[circularAppender.S :: "diskAddrs"] (slice_val diskaddrslice) ∗
+      is_slice_small diskaddrslice uint64T 1%Qp (u64val <$> (update.addr <$> updarray')) ∗
       updates_slice bufs upds ∗
-      is_circular_appender c circAppenderList ∗
-       (∀ σ σ' b,
-         ⌜relation.denote (circ_append upds newEnd circAppenderList) σ σ' b⌝ -∗
-         (P σ ={⊤ ∖↑ N}=∗ P σ' ∗ Q))
+      ⌜updarray' = apply_updates updarray (int.val endpos) upds⌝
+  }}}.
+Proof.
+  iIntros (Φ) "(#Hcirc & Hγ & Hdiskaddrs & Hslice & Hupdslice) HΦ".
+  wp_lam. wp_let. wp_let. wp_let.
+  iDestruct "Hupdslice" as (bks) "[Hupdslice Hbks]".
+
+  iDestruct (is_slice_small_sz with "Hupdslice") as %Hslen.
+  rewrite fmap_length in Hslen.
+  iDestruct (big_sepL2_length with "Hbks") as %Hslen2.
+
+  wp_apply (wp_forSlice (fun i =>
+    ∃ updarray',
+      own γ (◯ Excl' updarray') ∗
+      c ↦[circularAppender.S :: "diskAddrs"] (slice_val diskaddrslice) ∗
+      is_slice_small diskaddrslice uint64T 1%Qp (u64val <$> (update.addr <$> updarray')) ∗
+      ( [∗ list] b_upd;upd ∈ bks;upds, let '{| update.addr := a; update.b := b |} := upd in
+                                         is_block b_upd.2 b ∗ ⌜b_upd.1 = a⌝) ∗
+      ⌜updarray' = apply_updates updarray (int.val endpos) (firstn (int.nat i) upds)⌝)%I
+    with "[] [Hγ Hdiskaddrs Hslice Hupdslice Hbks]").
+
+  2: {
+    iFrame.
+    iExists _. iFrame. 
+    rewrite firstn_O /=. done.
+  }
+
+  2: {
+    iIntros "[Hloop Hupdslice]".
+    iDestruct "Hloop" as (updarray') "(Hγ & Hdiskaddrs & Hslice & Hbks & ->)".
+    iApply "HΦ".
+    iFrame.
+    iSplitL "Hbks Hupdslice".
+    { iExists _. iFrame. }
+    rewrite <- Hslen.
+    rewrite Hslen2.
+    rewrite firstn_all. done.
+  }
+
+  iIntros (i x Φloop) "!> (Hloop & % & %) HΦloop".
+  iDestruct "Hloop" as (updarray') "(Hγ & Hdiskaddrs & Hslice & Hbks & ->)".
+
+  wp_pures.
+
+  destruct (list_lookup_lt _ upds (int.nat i)).
+  { word. }
+  destruct (list_lookup_lt _ bks (int.nat i)).
+  { word. }
+  rewrite list_lookup_fmap in H1.
+  rewrite H3 in H1. simpl in H1. inversion H1; clear H1; subst.
+  destruct x1. destruct x0.
+
+  iDestruct (big_sepL2_lookup_acc with "Hbks") as "[Hi Hbks]"; eauto.
+  rewrite /=.
+  iDestruct "Hi" as "[Hi ->]".
+
+  rewrite /update_val /=.
+Admitted.
+
+Theorem wp_circular__Append (Q: iProp Σ) γ d (endpos : u64) (bufs : Slice.t) (upds : list update.t) c (circAppenderList : list u64) :
+  {{{ is_circular γ ∗
+      updates_slice bufs upds ∗
+      is_circular_appender γ c ∗
+      (∀ σ, P σ -∗
+        ( (∃ σ' b, ⌜relation.denote (circ_append upds endpos) σ σ' b⌝) ∧
+          (∀ σ' b, ⌜relation.denote (circ_append upds endpos) σ σ' b⌝ ={⊤ ∖↑ N}=∗ P σ' ∗ Q)))
   }}}
-    circularAppender__Append #c #d #newEnd (slice_val bufs)
+    circularAppender__Append #c #d #endpos (slice_val bufs)
   {{{ RET #(); Q }}}.
 Proof.
-  iIntros (Φ) "(#Hcirc & Hslice & Hfupd) HΦ".
+  iIntros (Φ) "(#Hcirc & Hslice & Hca & Hfupd) HΦ".
   wp_call.
+
+  iDestruct "Hca" as (addrslice updarray) "(Hγ & Haddrslice & Hs)".
+  wp_apply (wp_circularAppender__logBlocks with "[$Hcirc $Hslice $Hγ $Haddrslice $Hs]").
+
+  iIntros (updarray') "(Hγ & Haddrslice & Hs & Hupdslice & ->)".
+  wp_apply wp_slice_len.
+  wp_pures.
   wp_call.
+
+  wp_apply wp_new_enc.
+  iIntros (enc) "[Henc %]".
+  wp_apply (wp_Enc__PutInt with "[$Henc]").
+  {
+Transparent encode.
+    iPureIntro. rewrite /=. rewrite H0. word.
+Opaque encode.
+  }
+  iIntros "Henc".
+  wp_loadField.
+  wp_apply (wp_Enc__PutInts with "[$Henc $Hs]").
+  {
+Transparent encode.
+    iPureIntro. rewrite /=. rewrite H0. admit.
+Opaque encode.
+  }
+  iIntros "[Henc Hs]".
+
+  wp_apply (wp_Enc__Finish with "Henc").
+  iIntros (s extra) "[Hslice %]".
+
+  wp_apply (wp_Write_fupd _ Q with "[Hslice Hγ Hfupd]").
+  {
+    iDestruct (is_slice_small_sz with "Hslice") as %Hslen.
+    rewrite fmap_length in Hslen.
+
+    iSplitL "Hslice".
+    { rewrite -list_to_block_to_vals; first iFrame.
+      rewrite Hslen. rewrite H1. rewrite H0. word.
+    }
+
+    iInv N as ">Hcircopen" "Hclose".
+    iDestruct "Hcircopen" as (σ) "[Hcs HP]".
+    iDestruct "Hcs" as (updarray0) "(Hγauth & Hlow & Hupds)".
+    iDestruct "Hlow" as "[% Hlow]".
+    iDestruct "Hlow" as (hdr1 hdr2 hdr2extra) "(Hd0 & Hd1 & % & % & Hd2)".
+    iExists _. iFrame.
+    iModIntro.
+    iIntros "Hd0".
+
+    iDestruct (ghost_var_agree with "Hγauth Hγ") as %->.
+
+    iDestruct ("Hfupd" with "HP") as "[Hex Hfupd]".
+    iDestruct "Hex" as (eσ' eb) "Hex".
+    iDestruct "Hex" as %Hex.
+
+    iSpecialize ("Hfupd" $! eσ' eb).
+    simpl in Hex. monad_inv.
+
+    iDestruct ("Hfupd" with "[]") as "Hfupd".
+    { iPureIntro. repeat econstructor; lia. }
+
+    iMod "Hfupd" as "[HP HQ]". iFrame.
+    iApply "Hclose".
+
+    iNext. iExists _. iFrame.
+    iExists _. destruct σ. rewrite /=.
+    iSplitL "Hγauth"; first iFrame.
+    iSplitL "Hd0 Hd1 Hd2".
+    { rewrite /is_low_state. iSplitR "Hd0 Hd1 Hd2".
+      2: {
+        iExists _, _, _. iFrame.
+        iPureIntro; intuition idtac; simpl in *.
+        {
+          admit.
+        }
+        {
+          eauto.
+        }
+      }
+      done.
+    }
+    iFrame.
+    admit.
+  }
+
+  iIntros "[Hslice HQ]".
+  wp_pures.
+  wp_call.
+  iApply "HΦ".
+  iFrame.
 Admitted.
 
 End heap.
